Allow dependent products in CS.
This removes the restriction to non-dependent products. Note: It does 
*not* have a fast path for non-dependent products.

pretyping/evarconv.ml
@@ -244,12 +244,9 @@ let check_conv_record env sigma (t1,sk1) (t2,sk2) =
   let canon_s,sk2_effective =
     try
       match EConstr.kind sigma t2 with
-        Prod (_,a,b) -> (* assert (l2=[]); *)
-          let _, a, b = destProd sigma t2 in
-          if noccurn sigma 1 b then
+        Prod (_,_,_) -> (* assert (l2=[]); *)
             lookup_canonical_conversion (proji, Prod_cs),
-            (Stack.append_app [|a;pop b|] Stack.empty)
-          else raise Not_found
+            (Stack.append_app [|t2|] Stack.empty)
       | Sort s ->
         let s = ESorts.kind sigma s in
         lookup_canonical_conversion
